theories/Operational/Common/OSDelayAdapterContract.v
@@ -1,0 +1,145 @@
+From Stdlib Require Import List.
+From RocqSched Require Import Foundation.Base.
+From RocqSched Require Import Semantics.Schedule.
+From RocqSched Require Import Abstractions.Scheduler.Interface.
+From RocqSched Require Import Abstractions.SchedulingAlgorithm.Interface.
+From RocqSched Require Import Abstractions.SchedulingAlgorithm.SchedulerBridge.
+From RocqSched Require Import Abstractions.SchedulingAlgorithm.TopMInterface.
+From RocqSched Require Import Abstractions.SchedulingAlgorithm.TopMSchedulerBridge.
+From RocqSched Require Import Multicore.Common.MultiCoreBase.
+From RocqSched Require Import Multicore.Common.Admissibility.
+From RocqSched Require Import Multicore.Common.ValidityFacts.
+From RocqSched Require Import Operational.Common.DelayModel.
+From RocqSched Require Import Operational.Common.DelayBudget.
+From RocqSched Require Import Operational.Common.OSProjectionInterface.
+From RocqSched Require Import Operational.Common.LabeledExecution.
+From RocqSched Require Import Operational.Common.ConcreteExecution.
+From RocqSched Require Import Operational.Common.OSLocalAdapterContract.
+From RocqSched Require Import Operational.Common.OSAdapterContract.
+From RocqSched Require Import Operational.Common.OSCandidateSourceContract.
+From RocqSched Require Import Operational.Common.OSSchedulerRelationContract.
+From RocqSched Require Import Operational.Common.OSAlgorithmAdapterContract.
+From RocqSched Require Import Refinement.BoundedDelayRefinement.
+Import ListNotations.
+
+Record os_delay_adapter_contract
+    {CState : Type}
+    (P : OSLabeledProjection CState)
+    (jobs : JobId -> Job)
+    (adm : admissible_cpu)
+    (m : nat) : Type :=
+  mkOSDelayAdapterContract {
+    odac_base : os_multicore_adapter_contract P jobs adm m;
+    odac_ideal_schedule : Schedule;
+    odac_delay_bounds : op_delay_bounds;
+    odac_delay_sources : DelayTrace;
+    odac_delta : nat;
+    odac_ideal_valid :
+      multicore_semantic_validity jobs m odac_ideal_schedule;
+    odac_default_sources_covered :
+      forall t src,
+        In src
+           (default_event_delay_sources
+              (lex_event
+                 (concrete_to_labeled_execution (oac_execution odac_base)) t)) ->
+        In src (odac_delay_sources t);
+    odac_budget_within_delta :
+      forall t,
+        delay_budget_le
+          odac_delay_bounds
+          odac_delay_sources
+          0
+          t
+          odac_delta;
+    odac_service_lag :
+      service_lag_le
+        m
+        odac_ideal_schedule
+        (labeled_actual_schedule
+           (concrete_to_labeled_execution (oac_execution odac_base)))
+        odac_delta;
+  }.
+
+Definition projected_top_m_algorithm_execution
+    {CState : Type}
+    {P : OSLabeledProjection CState}
+    {J : JobId -> Prop}
+    {spec : GenericTopMSchedulingAlgorithm}
+    {candidates_of : CandidateSource}
+    {jobs : JobId -> Job}
+    {adm : admissible_cpu}
+    {m : nat}
+    (C : os_top_m_algorithm_adapter_contract
+           P J spec candidates_of jobs adm m)
+  : labeled_concrete_execution P m :=
+  olac_execution
+    (olcsac_base
+       (oltsrac_base
+          (otmaac_scheduler_relation C))).
+
+Record os_delay_top_m_adapter_contract
+    {CState : Type}
+    (P : OSLabeledProjection CState)
+    (J : JobId -> Prop)
+    (spec : GenericTopMSchedulingAlgorithm)
+    (candidates_of : CandidateSource)
+    (jobs : JobId -> Job)
+    (adm : admissible_cpu)
+    (m : nat) : Type :=
+  mkOSDelayTopMAdapterContract {
+    odtac_base :
+      os_top_m_algorithm_adapter_contract
+        P
+        J
+        spec
+        candidates_of
+        jobs
+        adm
+        m;
+    odtac_ideal_schedule : Schedule;
+    odtac_delay_bounds : op_delay_bounds;
+    odtac_delay_sources : DelayTrace;
+    odtac_delta : nat;
+    odtac_ideal_top_m :
+      scheduler_rel
+        (top_m_algorithm_schedule spec candidates_of)
+        jobs m odtac_ideal_schedule;
+    odtac_default_sources_covered :
+      forall t src,
+        In src
+           (default_event_delay_sources
+              (lex_event
+                 (concrete_to_labeled_execution
+                    (projected_top_m_algorithm_execution odtac_base))
+                 t)) ->
+        In src (odtac_delay_sources t);
+    odtac_budget_within_delta :
+      forall t,
+        delay_budget_le
+          odtac_delay_bounds
+          odtac_delay_sources
+          0
+          t
+          odtac_delta;
+    odtac_service_lag :
+      service_lag_le
+        m
+        odtac_ideal_schedule
+        (labeled_actual_schedule
+           (concrete_to_labeled_execution
+              (projected_top_m_algorithm_execution odtac_base)))
+        odtac_delta;
+  }.
+
+Arguments odac_base {CState P jobs adm m} _.
+Arguments odac_ideal_schedule {CState P jobs adm m} _.
+Arguments odac_delay_bounds {CState P jobs adm m} _.
+Arguments odac_delay_sources {CState P jobs adm m} _ _.
+Arguments odac_delta {CState P jobs adm m} _.
+Arguments odac_ideal_valid {CState P jobs adm m} _.
+Arguments odtac_base {CState P J spec candidates_of jobs adm m} _.
+Arguments odtac_ideal_schedule {CState P J spec candidates_of jobs adm m} _.
+Arguments odtac_delay_bounds {CState P J spec candidates_of jobs adm m} _.
+Arguments odtac_delay_sources {CState P J spec candidates_of jobs adm m} _ _.
+Arguments odtac_delta {CState P J spec candidates_of jobs adm m} _.
+Arguments odtac_ideal_top_m {CState P J spec candidates_of jobs adm m} _.
